examples/invariants/DY.Example.Invariants.Uniqueness.fst
@@ -6,6 +6,8 @@ module L = DY.Lib
 module List = FStar.List.Tot.Base
 module Trace = DY.Core.Trace.Type
 
+#set-options "--fuel 1 --ifuel 1"
+
 /// Experimenting with the new state invariants for sessions and full states
 
 type p_state =
@@ -82,21 +84,22 @@ let p_state_pred: state_predicate p_cinvs = {
       match parse p_state cont with
         | None -> False
         | Some (S the_idn _) -> begin     
-            forall sess. sess `List.mem` full_st_b ==>
-             ( match sess with
-               | (_, Nil) -> True
+            forall_sessions full_st_b
+            (fun sid_i sess_i -> 
+              match sess_i with
+              | Nil -> True            
                      // this should always be true (and we should hide it from the user)
                      // since this corresponds to [session_pred]
                      // one could also argue that empty sessions should not appear in the full state 
-               | (sid_i, Snoc init_i last_i) -> begin
+              | Snoc init_i last_i -> begin
                     match parse p_state last_i with
                     | None -> True
                     | Some last_i ->
                         if sid_i = sid // if the new state is added to session sid_i
                           then last_i.idn = the_idn // the id should stay the same within session sid_i
                           else last_i.idn <> the_idn // otherwise the id must be different
-                 end
-             )
+                end
+            )
         end
     )
   ; pred_later = (fun t1 t2 p sid cont -> ())
@@ -112,141 +115,108 @@ instance protocol_invariants_p: protocol_invariants = {
   }
 }
 
-#push-options "--z3rlimit 100 " // --z3cliopt 'smt.qi.eager_threshold=100'"
+let forall_sessions_intro 
+  (full_st: full_state_raw)
+  (p: state_id -> session_raw -> prop)
+  (pf: ( (sid:state_id) -> (sess:session_raw) -> squash ((sid,sess) `List.mem` full_st) -> Tot (squash ( p sid sess)) ))
+  : (squash ( forall_sessions full_st p ))
+= introduce forall sid sess. (sid, sess) `List.mem` full_st ==> p sid sess 
+  with  
+    introduce (sid, sess) `List.mem` full_st ==> p sid sess 
+    with _ . pf sid sess _
+    
+#push-options "--fuel 2 --z3rlimit 50 --z3cliopt 'smt.qi.eager_threshold=100'"
 val next_full_state_pred:
   tr:trace -> p:principal -> sid:state_id ->
   Lemma 
-    (requires trace_invariant tr)
-    (ensures  (
-      let (_,tr_out) = next p sid tr in
-      match get_state p sid tr with
-      | (None, _) -> True
-      | (Some oldst_b, _) -> (
-        match parse p_state oldst_b with
-        | None -> True
-        | Some (S idn c) -> (          
-            let msg = M p in
-            let msg_b = serialize message msg in
-            let (_, tr_after_msg) = send_msg msg_b tr in
+  (requires
+       trace_invariant tr
+     /\ has_state_for tr p sid
+     /\ Some? (parse p_state (access_state tr p sid))
+  )
+  (ensures (
+     let S idn c = Some?.v (parse p_state (access_state tr p sid)) in
+     let (_, tr_after_msg) = send_msg (serialize message (M p)) tr in
+     let (_, tr_after_next_state) = set_state p sid (serialize p_state (S idn (c+1))) tr_after_msg in
 
-            let next_state = S idn (c+1) in
-            let next_state_b = serialize p_state next_state in
-            let (_,tr_after_next_state) = set_state p sid next_state_b tr_after_msg in
-             match (get_full_state p tr_after_msg) with
-            | (None,_) -> True
-            | (Some full_st_b, _) -> full_state_pred tr_after_msg full_st_b p sid next_state_b
-          )
-        )
-    ))
-let next_full_state_pred tr p sid = 
-  match get_state p sid tr with
-  | (None, _) -> ()
-  | (Some oldst_b, _) -> (
-      match parse p_state oldst_b with
-      | None -> ()
-      | Some (S idn c) -> (          
-          let msg = M p in
-          let msg_b = serialize message msg in
-          let (_, tr_after_msg) = send_msg msg_b tr in
-          serialize_wf_lemma message (is_publishable tr) msg;
-          assert(trace_invariant tr_after_msg);
+       has_full_state_for tr_after_msg p
+     /\ full_state_pred tr_after_msg (access_full_state tr_after_msg p) p sid (serialize p_state (S idn (c+1)))
+  ))
+let next_full_state_pred tr p sid =
+  let oldst_b = access_state tr p sid in
+  let S idn c = Some?.v (parse p_state oldst_b) in
+  let msg = M p in
+  let (_, tr_after_msg) = send_msg (serialize message msg) tr in
 
-          let next_state = S idn (c+1) in
-          let next_state_b = serialize p_state next_state in
-          let (_,tr_after_next_state) = set_state p sid next_state_b tr_after_msg in
-          
-          match (get_full_state p tr_after_msg) with
-          | (None, _) -> ()
-          | (Some full_st_b, _) -> begin
-              introduce forall x. x `List.mem` full_st_b ==>
-                (match x with
-                | (_, Nil) -> True
-                | (sid_i, Snoc init_i last_i) -> (
-                    match parse p_state last_i with
-                    | None -> True
-                    | Some last_i ->
-                        if sid_i = sid 
-                          then last_i.idn = idn
-                          else last_i.idn <> idn
-                  )
-                  )
-              with begin
-              introduce x `List.mem` full_st_b ==> (match x with
-                | (_, Nil) -> True
-                | (sid_i, Snoc init_i last_i) -> (
-                    match parse p_state last_i with
-                    | None -> True
-                    | Some last_i ->
-                        if sid_i = sid 
-                          then last_i.idn = idn
-                          else last_i.idn <> idn
-                  )
-                  )
-              with _ . begin
-                  match x with
-                  | (_, Nil) -> ()
-                  | (sid_i, (Snoc init_i last_i_b)) ->
-                       match parse p_state last_i_b with
-                       | None -> ()
-                       | Some last_i -> 
-                           //full_state_some_get_session_get_state p sid_i tr_after_msg;
+  let next_state = S idn (c+1) in
+  let (_,tr_after_next_state) = set_state p sid (serialize p_state next_state) tr_after_msg in
 
-                           get_state_same p sid_i tr tr_after_msg;    
-                           full_state_mem_get_session_get_state_forall p tr_after_msg;
-                           assert(last_i_b = access_state tr_after_msg p sid_i);
-                           if sid_i = sid
-                           then assert(last_i = S idn c)
-                           else begin
-                             let oldst_entry = SetState p sid oldst_b in
-                             let tr_after_oldst = tr `suffix_after_event` oldst_entry in
-                             let last_i_entry = SetState p sid_i last_i_b in
-                             let tr_after_last_i = tr `suffix_after_event` last_i_entry in
-                             
-                             if tr_after_oldst `has_suffix` tr_after_last_i // last_i after oldst on tr
-                             then (admit();
-                               get_state_no_set_state_for_on_suffix_after_event tr p sid;
-                               no_set_state_entry_for_on_suffix tr_after_oldst tr_after_last_i p sid;
-                               assert(no_set_state_entry_for p sid tr_after_last_i);
+  get_state_appears_in_full_state tr p sid;
+  get_full_state_on_growing_traces p tr tr_after_msg sid;
+  assert(has_full_state_for tr_after_msg p);
+  let full_st_b = access_full_state tr_after_msg p in
+  forall_sessions_intro full_st_b
+    (fun sid_i sess_i -> 
+       match sess_i with
+       | Nil -> True
+       | Snoc init_i last_i -> (
+           match parse p_state last_i with
+           | None -> True
+           | Some last_i ->
+               if sid_i = sid 
+                 then last_i.idn = idn
+                 else last_i.idn <> idn
+         )
+    )
+    (fun sid_i sess_i _ ->
+       match sess_i with
+       | Nil -> ()
+       | Snoc init_i last_i_b ->
+            match parse p_state last_i_b with
+            | None -> ()
+            | Some last_i -> 
+                get_state_same p sid_i tr tr_after_msg;    
+                full_state_mem_get_session_get_state_forall p tr_after_msg;
+                assert(last_i_b = access_state tr_after_msg p sid_i);
+                if sid_i = sid
+                then assert(last_i = S idn c)
+                else (
+                  let oldst_entry = SetState p sid oldst_b in
+                  let tr_after_oldst = tr `suffix_after_event` oldst_entry in
+                  let last_i_entry = SetState p sid_i last_i_b in
+                  let tr_after_last_i = tr `suffix_after_event` last_i_entry in
 
-                               let tr_before_last_i = tr `prefix_before_event` (SetState p sid_i last_i_b) in
-                               suff_after_before_event_is_suff_at_event tr last_i_entry;
-                               no_set_state_entry_for_concat p sid (Snoc Nil (SetState p sid_i last_i_b)) tr_after_last_i;
-                               get_state_same p sid tr_before_last_i tr;
-                               assert(oldst_b = access_state tr_before_last_i p sid);
-                               // match get_full_state p tr_before_last_i with
-                               // | (None, _) -> get_state_appears_in_full_state tr_before_last_i p sid
-                               // | (Some full_state_before_last_i, _) -> (
-                                   prefix_before_event_invariant tr_after_msg (SetState p sid_i last_i_b);
-                                   assert(global_state_pred tr_before_last_i p sid_i last_i_b);
-                                   get_state_appears_in_full_state tr_before_last_i p sid 
-                                 // )
-                             )
-                             else ( // oldst after last_i on tr
-                               //admit();
-                               suffixes tr tr_after_last_i tr_after_oldst;
-                               assert(tr_after_last_i `has_suffix` tr_after_oldst);
-  
-                               get_state_no_set_state_for_on_suffix_after_event tr p sid_i;
-                               no_set_state_entry_for_on_suffix tr_after_last_i tr_after_oldst p sid_i;
-                               let tr_before_old = tr `prefix_before_event` oldst_entry in                               
-                               suff_after_before_event_is_suff_at_event tr oldst_entry;
-                               no_set_state_entry_for_concat p sid_i (Snoc Nil oldst_entry) tr_after_oldst;
-                               get_state_same p sid_i tr_before_old tr;
-                               let state_i_before_old = access_state tr_before_old p sid_i in
-                               assert(state_i_before_old = last_i_b);
-                               match get_full_state p tr_before_old with
-                               | (None, _) -> get_state_appears_in_full_state tr_before_old p sid_i
-                               | (Some full_state_before_old, _) -> 
-                                      assert(global_state_pred tr_before_old p sid oldst_b);
-                                      get_state_appears_in_full_state tr_before_old p sid_i  
-                             )
-                           end
-              end;
-            ()
-            end;
-          ()
-          end
-        )
+                  if tr_after_oldst `has_suffix` tr_after_last_i
+                  then ( // last_i after oldst on tr
+                    //admit();
+                    get_state_no_set_state_for_on_suffix_after_event tr p sid;
+                    no_set_state_entry_for_on_suffix tr_after_oldst tr_after_last_i p sid;
+                    assert(no_set_state_entry_for p sid tr_after_last_i);
+                    let tr_before_last_i = tr `prefix_before_event` (SetState p sid_i last_i_b) in
+                    suff_after_before_event_is_suff_at_event tr last_i_entry;
+                    no_set_state_entry_for_concat p sid (Snoc Nil (SetState p sid_i last_i_b)) tr_after_last_i;
+                    get_state_same p sid tr_before_last_i tr;
+                    assert(oldst_b = access_state tr_before_last_i p sid);
+                    assert(global_state_pred tr_before_last_i p sid_i last_i_b);
+                    get_state_appears_in_full_state tr_before_last_i p sid
+                  )
+                  else ( // oldst after last_i on tr
+                    // admit();
+                    suffixes tr tr_after_last_i tr_after_oldst;
+                    assert(tr_after_last_i `has_suffix` tr_after_oldst);
+
+                    get_state_no_set_state_for_on_suffix_after_event tr p sid_i;
+                    no_set_state_entry_for_on_suffix tr_after_last_i tr_after_oldst p sid_i;
+                    let tr_before_old = tr `prefix_before_event` oldst_entry in                               
+                    suff_after_before_event_is_suff_at_event tr oldst_entry;
+                    no_set_state_entry_for_concat p sid_i (Snoc Nil oldst_entry) tr_after_oldst;
+                    get_state_same p sid_i tr_before_old tr;
+                    let state_i_before_old = access_state tr_before_old p sid_i in
+                    assert(state_i_before_old = last_i_b);
+                    assert(global_state_pred tr_before_old p sid oldst_b);
+                    get_state_appears_in_full_state tr_before_old p sid_i  
+                  )
+                )
     )
 #pop-options
 
